Definitions/MapHeap.v
@@ -1,17 +1,25 @@
-(*From stdpp Require Import fin_maps fin_map_dom.
-From stdpp Require Import strings pmap *)
 From stdpp Require Import gmap.
+Require Import Definitions.GHeap.
 
-From Coq Require Import Ascii.
-Require Import Top0.Keys.
-Require Import Coq.FSets.FMapAVL.
-Module E := FMapAVL.Make (AsciiVars).
+Lemma H_same_key_1: 
+  forall l v (h : Heap), 
+    lookup (M:=gmap HeapKey HeapVal) l (<[ l:=v ]> h) = Some v.
+Proof.
+  intros.
+  rewrite lookup_insert_Some.
+  left. split; reflexivity.
+Qed. 
 
-Open Scope char_scope.
+Lemma H_same_key_2:
+  forall l1 l2 v h,
+    l1 = l2 -> 
+    lookup (M:=gmap HeapKey HeapVal) l1 h = Some v ->
+    lookup (M:=gmap HeapKey HeapVal) l1 (<[ l2:=v ]> h) = Some v.
+Proof.
+  intros.
+  rewrite H.
+  rewrite  lookup_insert_Some.
+  left. split; reflexivity.
+Qed.
 
 
-Lemma Test:
-  {[ "x":=3]} =@{gmap Ascii.ascii nat} ∅.
-Admitted.  
-
-Close Scope char_scope.
